src/tactics/FStar.Tactics.V2.Interpreter.fst
@@ -652,6 +652,10 @@ let () =
         refl_core_check_term RE.e_env RE.e_term RE.e_term E.e_tot_or_ghost (e_tuple2 (e_option e_unit) (e_list e_issue))
         refl_core_check_term NRE.e_env NRE.e_term NRE.e_term E.e_tot_or_ghost_nbe NBET.(e_tuple2 (e_option e_unit) (e_list e_issue));
 
+      mk_tac_step_3 0 "core_check_term_at_type"
+        refl_core_check_term_at_type RE.e_env RE.e_term RE.e_term (e_tuple2 (e_option E.e_tot_or_ghost) (e_list e_issue))
+        refl_core_check_term_at_type NRE.e_env NRE.e_term NRE.e_term NBET.(e_tuple2 (e_option  E.e_tot_or_ghost_nbe) (e_list e_issue));
+
       mk_tac_step_2 0 "tc_term"
         refl_tc_term RE.e_env RE.e_term (e_tuple2 (e_option (e_tuple2 RE.e_term (e_tuple2 E.e_tot_or_ghost RE.e_term))) (e_list e_issue))
         refl_tc_term NRE.e_env NRE.e_term NBET.(e_tuple2 (e_option (e_tuple2 NRE.e_term (e_tuple2 E.e_tot_or_ghost_nbe NRE.e_term))) (e_list e_issue));
